extra.v
@@ -1,0 +1,168 @@
+From mathcomp
+Require Import ssreflect ssrfun ssrbool eqtype ssrnat seq choice fintype tuple.
+From mathcomp
+Require Import bigop finset finfun perm fingraph path div.
+Require Import bigmin.
+
+Set Implicit Arguments.
+Unset Strict Implicit.
+Unset Printing Implicit Defensive.
+
+Section extra_div.
+
+Lemma ltn_div2r p m n : p > 0 -> m %/ p < n %/ p -> m < n.
+Proof.
+move=> p_gt0 lt_div; rewrite (divn_eq m p) (divn_eq n p).
+rewrite -(subnKC lt_div) mulnDl mulSn -!addnA addnCA ltn_add2l.
+by rewrite (leq_trans (ltn_pmod _ _)) // leq_addr.
+Qed.
+
+Lemma ltn_mod2r p m n : p > 0 -> m %/ p = n %/ p -> m %% p < n %% p -> m < n.
+Proof.
+move=> p_gt0 eq_div lt_mod; rewrite (divn_eq m p) (divn_eq n p).
+by rewrite {}eq_div ltn_add2l in lt_mod *.
+Qed.
+
+End extra_div.
+
+Section extra_seq.
+
+Lemma take_subseq (T : eqType) n (s : seq T) : subseq (take n s) s.
+Proof. by rewrite -[X in subseq _ X](cat_take_drop n) prefix_subseq. Qed.
+
+Lemma drop_subseq (T : eqType) n (s : seq T) : subseq (drop n s) s.
+Proof. by rewrite -[X in subseq _ X](cat_take_drop n) suffix_subseq. Qed.
+
+Lemma set_last_default (T : eqType) y0 x0 (s : seq T) :
+   size s > 0 -> last x0 s = last y0 s.
+Proof.
+by move=> s_gt0; rewrite -!nth_last; apply/set_nth_default; rewrite ?prednK.
+Qed.
+
+Lemma last_take (T : eqType) (x : T) n s :
+  last x (take n s) = if n == 0 then x
+                      else if n <= size s then nth x s n.-1 else last x s.
+Proof.
+elim: n s => [|n ihn] [|y s] //= in x *; rewrite {}ihn ltnS; case: n => //=.
+by move=> n; case: ltnP => // n_lt; apply/set_nth_default.
+Qed.
+
+Lemma last_drop (T : eqType) (x : T) n s :
+  last x (drop n s) = if n < size s then last x s else x.
+Proof.
+case: ltnP => sn; last by rewrite drop_oversize.
+rewrite -[s in RHS](cat_take_drop n) last_cat.
+by rewrite (@set_last_default _ x) ?size_drop ?subn_gt0.
+Qed.
+
+Lemma uniq_catLR (T : eqType) (x : T) s1 s2 : uniq (s1 ++ s2) ->
+  x \in s1 ++ s2 -> (x \in s1) = (x \notin s2).
+Proof.
+rewrite mem_cat=> s_uniq /orP[] x_in; move: s_uniq.
+  by rewrite uniq_catC cat_uniq => /and3P[_ /hasPn /(_ _ x_in)->].
+by rewrite cat_uniq => /and3P[_ /hasPn /(_ _ x_in) /= /negPf->]; rewrite x_in.
+Qed.
+
+Lemma uniq_catRL (T : eqType) (x : T) s1 s2 : uniq (s1 ++ s2) ->
+  x \in s1 ++ s2 -> uniq (s1 ++ s2) -> (x \in s2) = (x \notin s1).
+Proof.
+rewrite mem_cat uniq_catC => s_uniq x_s.
+by rewrite (uniq_catLR s_uniq) // mem_cat orbC.
+Qed.
+
+End extra_seq.
+
+Section extra_fintype.
+
+Lemma subset_cover (T: finType) (sccs sccs' : {set {set T}}) :
+  sccs \subset sccs' -> cover sccs \subset cover sccs'.
+Proof.
+move=> /subsetP subsccs; apply/subsetP=> x /bigcupP [scc /subsccs].
+by move=> scc' x_in; apply/bigcupP; exists scc.
+Qed.
+
+Lemma disjoint1s (T: finType) (A : pred T) (x : T) :
+   [disjoint [set x] & A] = (x \notin A).
+Proof.
+apply/pred0P/idP=> [/(_ x)/=|]; first by rewrite inE eqxx /= => ->.
+by move=> xNA y; rewrite !inE; case: eqP => //= ->; apply/negbTE.
+Qed.
+
+Lemma disjoints1 (T: finType) (A : pred T) (x : T) :
+   [disjoint A & [set x]] = (x \notin A).
+Proof. by rewrite disjoint_sym disjoint1s. Qed.
+
+End extra_fintype.
+
+Section extra_path.
+Variable (V : finType).
+
+Definition relto (a : pred V) (g : rel V) := [rel x y | (y \in a) && g x y].
+Definition relfrom (a : pred V) (g : rel V) := [rel x y | (x \in a) && g x y].
+
+Lemma connect_rev (g : rel V) :
+  connect g =2 (fun x => connect (fun x => g^~ x) ^~ x).
+Proof.
+move=> x y; apply/connectP/connectP=> [] [p gp ->].
+  exists (rev (belast x p)); rewrite ?rev_path //.
+  by case: (lastP p) => //= ??; rewrite belast_rcons rev_cons last_rcons.
+exists (rev (belast y p)); rewrite ?rev_path //.
+by case: (lastP p) => //= ??; rewrite belast_rcons rev_cons last_rcons.
+Qed.
+
+Lemma path_to a g z p : path (relto a g) z p = (path g z p) && (all a p).
+Proof.
+apply/(pathP z)/idP => [fgi|/andP[/pathP gi] /allP ga]; last first.
+  by move=> i i_lt /=; rewrite gi ?andbT ?[_ \in _]ga // mem_nth.
+rewrite (appP (pathP z) idP) //=; last by move=> i /fgi /= /andP[_ ->].
+by apply/(all_nthP z) => i /fgi /andP [].
+Qed.
+
+Lemma path_from a g z p :
+  path (relfrom a g) z p = (path g z p) && (all a (belast z p)).
+Proof. by rewrite -rev_path path_to all_rev rev_path. Qed.
+
+
+Lemma connect_to (a : pred V) (g : rel V) x z : connect g x z ->
+  exists y , [/\ (y \in a) ==> (x == y) && (x \in a),
+                 connect g x y & connect (relto a g) y z].
+Proof.
+move=> /connectP [p gxp ->].
+pose P := [pred i | let y := nth x (x :: p) i in
+  [&& connect g x y & connect (relto a g) y (last x p)]].
+have [] := @ex_minnP P.
+  by exists (size p); rewrite /= nth_last (path_connect gxp) //= mem_last.
+move=> i /= /andP[g1 g2] i_min; exists (nth x (x :: p) i); split=> //.
+case: i => [|i] //= in g1 g2 i_min *; first by rewrite eqxx /= implybb.
+have i_lt : i < size p.
+  by rewrite i_min // !nth_last /= (path_connect gxp) //= mem_last.
+have [<-/=|neq_xpi /=] := altP eqP; first by rewrite implybb.
+have := i_min i; rewrite ltnn => /contraNF /(_ isT) <-; apply/implyP=> axpi.
+rewrite (connect_trans _ g2) ?andbT //; last first.
+  by rewrite connect1 //= [_ \in _]axpi /= (pathP x _).
+by rewrite (path_connect gxp) //= mem_nth //= ltnW.
+Qed.
+
+Lemma connect_from (a : pred V) (g : rel V) x z : connect g x z ->
+  exists y, [/\ (y \in a) ==> (z == y) && (z \in a),
+                connect (relfrom a g) x y & connect g y z].
+Proof.
+rewrite connect_rev => cgxz; have [y [ayaz]]//= := connect_to a cgxz.
+by exists y; split; rewrite // connect_rev.
+Qed.
+
+Lemma connect1l (g : rel V) x z :
+  connect g x z -> z != x -> exists2 y, g x y & connect g y z.
+Proof.
+move=> /connectP [[|y p] //= xyp ->]; first by rewrite eqxx.
+by move: xyp=> /andP[]; exists y => //; apply/connectP; exists p.
+Qed.
+
+Lemma connect1r (g : rel V) x z :
+  connect g x z -> z != x -> exists2 y, connect g x y & g y z.
+Proof.
+move=> xz zNx; move: xz; rewrite connect_rev => /connect1l.
+by rewrite eq_sym => /(_ zNx) [y]; exists y; rewrite // connect_rev.
+Qed.
+
+End extra_path.
